Validate spill-base block generation

venom/codegen/proofs/spillBaseValidationScript.sml
@@ -155,3 +155,194 @@ Theorem spill_base_spilling_entry_succ_eval:
 Proof
   EVAL_TAC
 QED
+
+Definition spill_base_after_producer_def:
+  spill_base_after_producer b =
+    <| ps_stack :=
+         [Var "p17"; Var "p1"; Var "p2"; Var "p3"; Var "p4";
+          Var "p5"; Var "p6"; Var "p7"; Var "p8"; Var "p9";
+          Var "p10"; Var "p11"; Var "p12"; Var "p13"; Var "p14";
+          Var "p15"; Var "p16"; Var "p0"];
+       ps_spilled := FEMPTY;
+       ps_alloc :=
+         <| sa_free_slots :=
+              [b; b + 32; b + 64; b + 96; b + 128; b + 160;
+               b + 192; b + 224; b + 256; b + 288; b + 320;
+               b + 352; b + 384; b + 416; b + 448; b + 480;
+               b + 512; b + 544];
+            sa_next_offset := b + 576;
+            sa_spill_base := b |>;
+       ps_label_counter := 0 |>
+End
+
+Definition spill_base_producer_ops_def:
+  spill_base_producer_ops b =
+    [SOEmit "ADD";
+     SOSpill b; SOSpill (b + 32); SOSpill (b + 64); SOSpill (b + 96);
+     SOSpill (b + 128); SOSpill (b + 160); SOSpill (b + 192);
+     SOSpill (b + 224); SOSpill (b + 256); SOSpill (b + 288);
+     SOSpill (b + 320); SOSpill (b + 352); SOSpill (b + 384);
+     SOSpill (b + 416); SOSpill (b + 448); SOSpill (b + 480);
+     SOSpill (b + 512); SOSpill (b + 544);
+     SORestore b; SORestore (b + 512); SORestore (b + 480);
+     SORestore (b + 448); SORestore (b + 416); SORestore (b + 384);
+     SORestore (b + 352); SORestore (b + 320); SORestore (b + 288);
+     SORestore (b + 256); SORestore (b + 224); SORestore (b + 192);
+     SORestore (b + 160); SORestore (b + 128); SORestore (b + 96);
+     SORestore (b + 64); SORestore (b + 32); SORestore (b + 544)]
+End
+
+Theorem spill_base_producer_160_eval:
+  generate_inst_plan spill_base_spilling_live spill_base_spilling_dfg
+    spill_base_spilling_cfg spill_base_spilling_fn spill_base_producer
+    ["p17"; "p16"; "p15"; "p14"; "p13"; "p12"; "p11"; "p10";
+     "p9"; "p8"; "p7"; "p6"; "p5"; "p4"; "p3"; "p2"; "p1"; "p0"]
+    T F "entry" (init_plan_state 160) =
+  SOME (spill_base_producer_ops 160, spill_base_after_producer 160)
+Proof
+  EVAL_TAC >> simp[listTheory.SET_TO_LIST_EMPTY]
+QED
+
+
+Theorem spill_base_producer_224_eval:
+  generate_inst_plan spill_base_spilling_live spill_base_spilling_dfg
+    spill_base_spilling_cfg spill_base_spilling_fn spill_base_producer
+    ["p17"; "p16"; "p15"; "p14"; "p13"; "p12"; "p11"; "p10";
+     "p9"; "p8"; "p7"; "p6"; "p5"; "p4"; "p3"; "p2"; "p1"; "p0"]
+    T F "entry" (init_plan_state 224) =
+  SOME (spill_base_producer_ops 224, spill_base_after_producer 224)
+Proof
+  EVAL_TAC >> simp[listTheory.SET_TO_LIST_EMPTY]
+QED
+
+Definition spill_base_after_consumer_def:
+  spill_base_after_consumer b =
+    <| ps_stack := [];
+       ps_spilled := FEMPTY;
+       ps_alloc :=
+         <| sa_free_slots :=
+              [b; b + 32; b + 64; b + 96; b + 128; b + 160;
+               b + 192; b + 224; b + 256; b + 288; b + 320;
+               b + 352; b + 384; b + 416; b + 448; b + 480;
+               b + 512; b + 544];
+            sa_next_offset := b + 576;
+            sa_spill_base := b |>;
+       ps_label_counter := 0 |>
+End
+
+Definition spill_base_consumer_ops_def:
+  spill_base_consumer_ops =
+    [SOSwap 1; SOSwap 16; SOSwap 2; SOSwap 15; SOSwap 3; SOSwap 14;
+     SOSwap 4; SOSwap 13; SOSwap 5; SOSwap 12; SOSwap 6; SOSwap 11;
+     SOSwap 7; SOSwap 10; SOSwap 8; SOSwap 9; SOSwap 8; SOSwap 7;
+     SOSwap 6; SOSwap 5; SOSwap 4; SOSwap 3; SOSwap 2; SOEmit "ADD"]
+End
+
+Theorem spill_base_consumer_160_eval:
+  generate_inst_plan spill_base_spilling_live spill_base_spilling_dfg
+    spill_base_spilling_cfg spill_base_spilling_fn spill_base_consumer
+    [] T T "entry" (spill_base_after_producer 160) =
+  SOME (spill_base_consumer_ops, spill_base_after_consumer 160)
+Proof
+  EVAL_TAC >> simp[listTheory.SET_TO_LIST_EMPTY]
+QED
+
+Theorem spill_base_consumer_224_eval:
+  generate_inst_plan spill_base_spilling_live spill_base_spilling_dfg
+    spill_base_spilling_cfg spill_base_spilling_fn spill_base_consumer
+    [] T T "entry" (spill_base_after_producer 224) =
+  SOME (spill_base_consumer_ops, spill_base_after_consumer 224)
+Proof
+  EVAL_TAC >> simp[listTheory.SET_TO_LIST_EMPTY]
+QED
+
+Theorem spill_base_stop_160_eval:
+  generate_inst_plan spill_base_spilling_live spill_base_spilling_dfg
+    spill_base_spilling_cfg spill_base_spilling_fn spill_base_stop
+    [] T F "entry" (spill_base_after_consumer 160) =
+  SOME ([SOEmit "STOP"], spill_base_after_consumer 160)
+Proof
+  EVAL_TAC >> simp[listTheory.SET_TO_LIST_EMPTY]
+QED
+
+Theorem spill_base_stop_224_eval:
+  generate_inst_plan spill_base_spilling_live spill_base_spilling_dfg
+    spill_base_spilling_cfg spill_base_spilling_fn spill_base_stop
+    [] T F "entry" (spill_base_after_consumer 224) =
+  SOME ([SOEmit "STOP"], spill_base_after_consumer 224)
+Proof
+  EVAL_TAC >> simp[listTheory.SET_TO_LIST_EMPTY]
+QED
+
+Definition spill_base_block_ops_def:
+  spill_base_block_ops b =
+    SOLabel "entry" ::
+      (spill_base_producer_ops b ++ spill_base_consumer_ops ++
+       [SOEmit "STOP"])
+End
+
+Theorem spill_base_block_control_eval:
+  HD spill_base_spilling_fn.fn_blocks = spill_base_entry_bb /\
+  spill_base_entry_bb.bb_label = "entry" /\
+  spill_base_entry_bb.bb_instructions =
+    [spill_base_producer; spill_base_consumer; spill_base_stop] /\
+  prepare_params_plan spill_base_spilling_live spill_base_spilling_fn
+    (init_plan_state 160) = ([], init_plan_state 160) /\
+  prepare_params_plan spill_base_spilling_live spill_base_spilling_fn
+    (init_plan_state 224) = ([], init_plan_state 224) /\
+  cfg_preds_of spill_base_spilling_cfg "entry" = [] /\
+  non_param_insts spill_base_entry_bb =
+    [spill_base_producer; spill_base_consumer; spill_base_stop] /\
+  bb_is_halting spill_base_entry_bb /\
+  get_params spill_base_entry_bb.bb_instructions = [] /\
+  live_vars_at spill_base_spilling_live "entry" 1 =
+    ["p17"; "p16"; "p15"; "p14"; "p13"; "p12"; "p11"; "p10";
+     "p9"; "p8"; "p7"; "p6"; "p5"; "p4"; "p3"; "p2"; "p1"; "p0"] /\
+  live_vars_at spill_base_spilling_live "entry" 2 = [] /\
+  live_vars_at spill_base_spilling_live "entry" 3 = [] /\
+  ~is_terminator spill_base_consumer.inst_opcode /\
+  is_terminator spill_base_stop.inst_opcode
+Proof
+  EVAL_TAC >>
+  simp[livenessDefsTheory.live_vars_at_def, dfAnalyzeDefsTheory.df_at_def,
+       finite_mapTheory.FLOOKUP_UPDATE]
+QED
+
+Theorem spill_base_block_160_eval:
+  generate_block_plan spill_base_spilling_live spill_base_spilling_dfg
+    spill_base_spilling_cfg spill_base_spilling_fn spill_base_entry_bb
+    (init_plan_state 160) =
+  SOME (spill_base_block_ops 160, spill_base_after_consumer 160)
+Proof
+  simp[generate_block_plan_def, spill_base_block_control_eval,
+       spill_base_producer_160_eval, spill_base_consumer_160_eval,
+       spill_base_stop_160_eval, spill_base_block_ops_def]
+QED
+
+Theorem spill_base_block_224_eval:
+  generate_block_plan spill_base_spilling_live spill_base_spilling_dfg
+    spill_base_spilling_cfg spill_base_spilling_fn spill_base_entry_bb
+    (init_plan_state 224) =
+  SOME (spill_base_block_ops 224, spill_base_after_consumer 224)
+Proof
+  simp[generate_block_plan_def, spill_base_block_control_eval,
+       spill_base_producer_224_eval, spill_base_consumer_224_eval,
+       spill_base_stop_224_eval, spill_base_block_ops_def]
+QED
+
+
+Theorem spill_base_block_160_observables:
+  MEM (SOSpill 160) (spill_base_block_ops 160) /\
+  (spill_base_after_consumer 160).ps_alloc.sa_spill_base = 160 /\
+  160 < (spill_base_after_consumer 160).ps_alloc.sa_next_offset
+Proof
+  EVAL_TAC
+QED
+
+Theorem spill_base_block_224_observables:
+  MEM (SOSpill 224) (spill_base_block_ops 224) /\
+  (spill_base_after_consumer 224).ps_alloc.sa_spill_base = 224 /\
+  224 < (spill_base_after_consumer 224).ps_alloc.sa_next_offset
+Proof
+  EVAL_TAC
+QED
